---
aliases:
  - Sum Rule
  - Difference Rule
  - Constant Rule
  - Constant Multiple Rule
---
1. **[[Power Rule]]**
2. **Constant Rule**
   - If$f(x) = c$ (where $c$ is a constant), then$f'(x) = 0$.
3. **Constant Multiple Rule**
   - If$f(x) = c \cdot g(x)$(where $c$ is a constant), then$f'(x) = c \cdot g'(x)$.
4. **Sum Rule**
   - If$f(x) = g(x) + h(x)$, then$f'(x) = g'(x) + h'(x)$.
5. **Difference Rule**
   - If$f(x) = g(x) - h(x)$, then$f'(x) = g'(x) - h'(x)$.
6. **[[Product Rule]]**
7. **[[Quotient Rule]]**
8. **[[Chain Rule]]**